1) wf_phi_operands only checks if the incoming id is defined in a block   when the incoming block is reachable.
2) proved that substitution preserves WF. The proofs of substituting
variables and substituting constants in subst.v are same except the
wf_insn_base and wf_phi_operands cases. Vminus's proofs should be
simplied in the same way.

We also extended the Vminus's proof to allow substituting a variable
defined by a phinode. LAS/LAA do not need this, since they only
substitute variables defined by commands. The phinode-elimination pass
needs the extension.

3) proved that substitution preserves promotablity except one issue
  We may want to show that in the promotable alloca
    %p = alloca ty %num al
  the %num does not contain the variable (a load from %p) to be substed.
  This is definitely true, because %p must dominates the load, and the
  load cannot dominate %p.

  But, we may not have to show LAS/LAA preserve %num syntatically. First, 
  we have shown LAS/LAA back-simulate. Second, we only require that
  [|%num|] is positive. So, %num can be substituted (although
  impossible). We will delay the proof to see if removal also needs the
  property.

4) Fixed one bug in opsem_dom.v, which is same to a fixed problem in
opsem_wf.v (See r3387). opsem_dom.v is never used in mem2reg, so, did
not affect the proofs. opsem_dom.v is to prove GVN.



git-svn-id: https://webdav.seas.upenn.edu/svn/sol/vol@3967 eef5ea85-cc2e-0410-bd84-0fae1f012da8

src3.0/Vellvm/analysis.v
@@ -2850,7 +2850,7 @@ Inductive wf_phi_operands (f:fdef) (b:block) (id0:id) (t0:typ) :
     lookupBlockViaLabelFromFdef f l1 = Some b1 ->
     (((exists vb, lookupBlockViaIDFromFdef f vid1 = Some vb /\ 
        blockDominates f vb b1) \/ 
-      not (isReachableFromEntry f b)) \/ 
+      not (isReachableFromEntry f b1)) \/ 
      In vid1 (getArgsIDsOfFdef f)) ->
     wf_phi_operands f b id0 t0 vls ->
     wf_phi_operands f b id0 t0 ((value_id vid1, l1) :: vls)
